extending the StAE test, with one CT failure to investigate

src/tls/Test.StAE.fst
@@ -31,8 +31,17 @@ open StAE
 *)
 
 let prefix = "Test.StAE"
-let eprint s = FStar.HyperStack.IO.print_string (prefix^": ERROR: "^s^"\n")
-let nprint s = FStar.HyperStack.IO.print_string (prefix^": "^s^"\n")
+
+val discard: bool -> ST unit
+  (requires (fun _ -> True))
+  (ensures (fun h0 _ h1 -> h0 == h1))
+let discard _ = ()
+let print s = discard (IO.debug_print_string (prefix^": "^s^".\n"))
+// let print = C.String,print
+// let print = FStar.HyperStack.IO.print_string
+
+let eprint s = print ("ERROR: "^s)
+let nprint s = print s
 
 private let pre_id (role:role) =
   let cr  = Bytes.create 32ul 0z in
@@ -45,9 +54,24 @@ private let pre_id (role:role) =
   let msid = StandardMS pms (cr @| sr) kdf in
   ID12 TLS_1p2 msid kdf (AEAD CoreCrypto.AES_256_GCM Hashing.Spec.SHA256) cr sr role
 
-private let id = pre_id Client
+private let id12 = pre_id Client
 
 #set-options "--lax"
+
+private let id13 = 
+  let cr  = Bytes.create 32ul 0z in
+  let ch0 = { 
+    li_ch0_cr = cr; 
+    li_ch0_ed_psk = Bytes.utf8_encode "whatever"; 
+    li_ch0_ed_ae = CoreCrypto.AES_256_GCM;
+    li_ch0_ed_hash = Hashing.Spec.SHA256; } in
+  let li = LogInfo_CH0 ch0 in
+  let i = ExpandedSecret 
+      (EarlySecretID (NoPSK Hashing.Spec.SHA256)) 
+      ClientEarlyTrafficSecret 
+      (Bytes.utf8_encode "whatever") in
+  let kid: keyId = KeyID #li i in
+  ID13 kid
 
 private let encryptRecord (#id:StAE.stae_id) (wr:StAE.writer id) ct plain : St bytes =
   let rg: Range.frange id = (0, length plain) in
@@ -61,34 +85,68 @@ private let decryptRecord (#id:StAE.stae_id) (rd:StAE.reader id) ct cipher : St 
   | Some d -> Some (Content.repr id d)
   | _ -> None
 
-private let text = Bytes.utf8_encode "Top secret"
 
-val main : unit -> St C.exit_code
-let main() = 
-  //let wr = StAE.gen root id in
+val test: id:StAE.stae_id -> St bool
+let test id = 
+  let text0 = Bytes.utf8_encode "attack at" in 
+  let text1 = Bytes.utf8_encode "dawn" in
 
   // For TLS 1.2, key materials consist of an AES256 key plus 4 bytes of IV salt.
-  let key = bytes_of_hex ("feffe9928665731c6d6a8f9467308308feffe9928665731c6d6a8f9467308308" ^ "01020304") in
+  let key = 
+    if ID13? id then 
+    bytes_of_hex (
+    "feffe9928665731c6d6a8f9467308308feffe9928665731c6d6a8f9467308308"^
+    "0123456789abcdef0123456789abcdef0123456789abcdef0123456789abcdef") 
+    else
+    bytes_of_hex (
+    "feffe9928665731c6d6a8f9467308308feffe9928665731c6d6a8f9467308308"^
+    "01020304") 
+    in
   let wr = StAE.coerce root id key in
   let rd = StAE.genReader root #id wr in
-  let ct = Content.Application_data in
-  let c = encryptRecord #id wr ct text in
-  //print_string ("Encrypted: " ^ (iutf8 c) ^ "\n");
-  let d = decryptRecord #id rd ct c in
-  match d with
-  | None -> 
-      eprint ("decryption failed.\n");
-      C.EXIT_FAILURE 
-  | Some text' ->
-    if not(text = text') then (
-      eprint ("wrong decrypted message.\n");
-      eprint("  expected "^Bytes.hex_of_bytes text^ "\n");
-      eprint ("  decrypted "^Bytes.hex_of_bytes text'^"\n");
-      C.EXIT_FAILURE)
-    else (
-      nprint ("OK.\n");
-      C.EXIT_SUCCESS )
+   
+  let c0 = encryptRecord #id wr Content.Application_data text0 in
+  // how to print bytes? nprint("first encryption is "^c0)
+  let c1 = encryptRecord #id wr Content.Application_data text1 in
+
+  nprint "start";
+  (
+    let c = Bytes.utf8_encode "we need a long-enough ciphertext (static pre)" in 
+    let d = decryptRecord #id rd Content.Application_data c in
+    if None? d   
+    then (nprint "decryption fails on wrong cipher"; true)
+    else (eprint "decryption should fail"; false)
+  ) &&
+  ( let d = decryptRecord #id rd Content.Application_data c1 in
+    if None? d   
+    then (nprint "decryption fails on wrong sequence number"; true)
+    else (eprint "decryption should fail on wrong sequence number"; false)
+  ) &&
+  ( let d = decryptRecord #id rd Content.Alert c0 in
+    if None? d   
+    then (nprint "decryption fails on wrong CT"; true)
+    else (eprint "decryption should fail on wrong CT"; false)
+  ) &&
+  ( let d = decryptRecord #id rd Content.Application_data c0 in 
+    match d with 
+    | Some v ->
+      if v = text0 
+      then (nprint "first decryption succeeds"; true)
+      else (eprint "wrong decrypted message"; false)
+    | _ -> eprint ("decryption failed");  false 
+  ) &&
+  ( let d = decryptRecord #id rd Content.Application_data c1 in 
+    match d with 
+    | Some v ->
+      if v = text1 
+      then (nprint "second decryption succeeds"; true)
+      else (eprint "wrong decrypted message"; false)
+    | _ -> eprint ("decryption failed");  false )
+
+// will need to move to a Kremlin-specific driver
+let main() = 
+  if test id12 && test id13 then C.EXIT_SUCCESS else C.EXIT_FAILURE 
 
 // will need to move to an Ocaml-specific driver
 let _ = 
-  if main() = C.EXIT_FAILURE then failwith prefix else ()
+  if test id12 && test id13 then () else failwith prefix
